Finperm/Congr.lean
@@ -11,48 +11,80 @@ public import Finperm.MinPerm
 
 namespace Finperm
 
-@[irreducible] def IsCongr {n m : Nat} (a : Finperm n) (b : Finperm m) : Prop :=
-  (∀ i (hin : i < n) (him : i < m), a[i] = b[i]) ∧
-    (∀ i, ∀ (hi : i < n), m ≤ i → a[i] = i) ∧
-    (∀ i, ∀ (hi : i < m), n ≤ i → b[i] = i)
+def IsCongr {n m : Nat} (a : Finperm n) (b : Finperm m) : Prop :=
+  (∃ (h : n ≤ m), a.castGE h = b) ∨ (∃ (h : m ≤ n), b.castGE h = a)
 
 section IsCongr
 
 variable {n m l i : Nat} {a : Finperm n} {b : Finperm m} {c : Finperm l}
 
-unseal IsCongr in theorem isCongr_def :
+theorem isCongr_pointwise :
     a.IsCongr b ↔ (∀ i (hin : i < n) (him : i < m), a[i] = b[i]) ∧
     (∀ i, ∀ (hi : i < n), m ≤ i → a[i] = i) ∧
-    (∀ i, ∀ (hi : i < m), n ≤ i → b[i] = i) := Iff.rfl
+    (∀ i, ∀ (hi : i < m), n ≤ i → b[i] = i) := by
+  unfold IsCongr
+  simp only [Finperm.ext_iff, getElem_castGE]
+  grind
+
+theorem IsCongr.eq_castGE_of_le (h : n ≤ m) (hab : a.IsCongr b) : a.castGE h = b :=
+  hab.elim (fun ⟨_, h⟩ => h) (fun ⟨hnm, h⟩ => h ▸ by simp)
+
+theorem IsCongr.eq_castGE_of_ge (h : m ≤ n) (hab : a.IsCongr b) : b.castGE h = a :=
+  hab.elim (fun ⟨hnm, h⟩ => h ▸ by simp) (fun ⟨_, h⟩ => h)
+
+theorem isCongr_of_castGE_eq_right (h : n ≤ m) (hab : a.castGE h = b) : a.IsCongr b :=
+  Or.inl ⟨_, hab⟩
+
+theorem isCongr_of_castGE_eq_left (h : m ≤ n) (hab : b.castGE h = a) : a.IsCongr b :=
+  Or.inr ⟨_, hab⟩
+
+@[simp] theorem isCongr_castGE {h : n ≤ k} : a.IsCongr (a.castGE h) := Or.inl ⟨h, rfl⟩
+
+grind_pattern isCongr_castGE => a.castGE h
+
+@[simp] theorem castGE_isCongr {h : n ≤ k} : (a.castGE h).IsCongr a := Or.inr ⟨h, rfl⟩
+
+grind_pattern castGE_isCongr => a.castGE h
+
+@[simp, grind =] theorem castGE_eq_iff {h : n ≤ k} {h'} :
+    a.castGE h = b.castGE h' ↔ a.IsCongr b := by
+  simp only [Finperm.ext_iff, getElem_castGE, isCongr_pointwise]
+  grind
+
+@[simp, grind =] theorem isCongr_castGE_castGE_iff {h : n ≤ k} {h' : m ≤ o} :
+    (a.castGE h).IsCongr (b.castGE h') ↔ a.IsCongr b := by
+  simp only [isCongr_pointwise, getElem_castGE, dite_eq_right_iff]
+  grind
 
 instance {a : Finperm n} {b : Finperm m} : Decidable (a.IsCongr b) :=
-  decidable_of_decidable_of_iff isCongr_def.symm
+  decidable_of_decidable_of_iff isCongr_pointwise.symm
 
-@[simp, grind =] theorem isCongr_iff_eq {a' : Finperm n} : a.IsCongr a' ↔ a = a' := by
-  grind [isCongr_def]
+theorem IsCongr.eq {a' : Finperm n} (h : a.IsCongr a') : a = a' :=
+  (h.eq_castGE_of_ge n.le_refl).symm.trans a'.castGE_refl
 
-@[grind →] theorem IsCongr.symm : a.IsCongr b → b.IsCongr a := by grind [isCongr_def]
-
-@[grind →] theorem IsCongr.trans : a.IsCongr b → b.IsCongr c → a.IsCongr c := by
-  grind [isCongr_def]
-
-@[simp, grind =] theorem isCongr_one_iff : a.IsCongr (1 : Finperm m) ↔ a = 1 := by
-  grind [isCongr_def]
-
-@[grind →] theorem IsCongr.inv_inv : a.IsCongr b → a⁻¹.IsCongr b⁻¹ := by grind [isCongr_def]
-
-theorem IsCongr.mul_mul {a' : Finperm n} {b' : Finperm m} (hab : a.IsCongr b)
-    (hab' : a'.IsCongr b') : (a * a').IsCongr (b * b') := by grind [isCongr_def]
-
-grind_pattern IsCongr.mul_mul => a * a', b * b'
-
-theorem IsCongr.eq {a' : Finperm n} (h : a.IsCongr a') : a = a' := by grind
-
-@[simp] theorem isCongr_refl (a : Finperm n) : a.IsCongr a := by grind
+@[simp] theorem isCongr_refl (a : Finperm n) : a.IsCongr a :=
+  isCongr_of_castGE_eq_right n.le_refl a.castGE_refl
 
 theorem isCongr_rfl : a.IsCongr a := isCongr_refl a
 
+@[simp, grind =] theorem isCongr_iff_eq {a' : Finperm n} : a.IsCongr a' ↔ a = a' :=
+  ⟨IsCongr.eq, Eq.rec a.isCongr_refl⟩
+
+@[grind →] theorem IsCongr.symm (hab : a.IsCongr b) : b.IsCongr a := hab.elim Or.inr Or.inl
+
 theorem isCongr_comm : a.IsCongr b ↔ b.IsCongr a := by grind
+
+@[grind →] theorem IsCongr.trans (hab : a.IsCongr b) (hbc : b.IsCongr c) : a.IsCongr c := by
+  rcases hab <;> rcases hbc <;> grind
+
+@[grind →] theorem IsCongr.inv_inv : a.IsCongr b → a⁻¹.IsCongr b⁻¹ :=
+  Or.imp (Exists.imp <| by simp) (Exists.imp <| by simp)
+
+theorem IsCongr.mul_mul {a' : Finperm n} {b' : Finperm m} (hab : a.IsCongr b)
+    (hab' : a'.IsCongr b') : (a * a').IsCongr (b * b') := by
+  rcases hab  <;> rcases hab' <;> grind
+
+grind_pattern IsCongr.mul_mul => a * a', b * b'
 
 theorem IsCongr.congr (hab : a.IsCongr a') (hab' : b.IsCongr b') :
     a.IsCongr b ↔ a'.IsCongr b' := by grind
@@ -61,9 +93,19 @@ theorem IsCongr.congrLeft (hab : a.IsCongr b) : a.IsCongr c ↔ b.IsCongr c := b
 
 theorem IsCongr.congrRight (hab : a.IsCongr b) : c.IsCongr a ↔ c.IsCongr b := by grind
 
-@[simp] theorem one_isCongr_iff : (1 : Finperm m).IsCongr a ↔ a = 1 := by grind
+@[grind .]
+theorem isCongr_one_one : (1 : Finperm n).IsCongr (1 : Finperm m) :=
+  (Nat.le_or_ge n m).elim (fun _ => .inl (by grind)) (fun _ => .inr (by grind))
 
-theorem isCongr_one_one : (1 : Finperm n).IsCongr (1 : Finperm m) := by grind
+@[grind =>] theorem IsCongr.eq_one (ha : a.IsCongr (1 : Finperm m)) : a = 1 := by
+  rcases ha <;> grind
+
+@[grind =>] theorem IsCongr.one_eq (ha : (1 : Finperm m).IsCongr a) : 1 = a := by
+  rcases ha <;> grind
+
+@[simp] theorem isCongr_one_iff : a.IsCongr (1 : Finperm m) ↔ a = 1 := by grind
+
+@[simp] theorem one_isCongr_iff : (1 : Finperm m).IsCongr a ↔ a = 1 := by grind
 
 theorem IsCongr.inv_right (hab : a.IsCongr b⁻¹) : a⁻¹.IsCongr b := by grind
 
@@ -73,7 +115,6 @@ theorem inv_isCongr_iff_isCongr_inv : a⁻¹.IsCongr b ↔ a.IsCongr b⁻¹ := b
 
 @[simp] theorem inv_isCongr_inv_iff : a⁻¹.IsCongr b⁻¹ ↔ a.IsCongr b := by grind
 
-
 @[simp] theorem isCongr_cast {h : n = m} : a.IsCongr (a.cast h) := by subst h; simp
 
 grind_pattern isCongr_cast => a.cast h
@@ -82,17 +123,9 @@ grind_pattern isCongr_cast => a.cast h
 
 grind_pattern cast_isCongr => a.cast h
 
-@[simp] theorem isCongr_castGE {h : n ≤ k} : a.IsCongr (a.castGE h) := by grind [isCongr_def]
-
-grind_pattern isCongr_castGE => a.castGE h
-
-@[simp] theorem castGE_isCongr {h : n ≤ k} : (a.castGE h).IsCongr a := a.isCongr_castGE.symm
-
-grind_pattern castGE_isCongr => a.castGE h
-
 theorem IsCongr.hmul_hmul {a' : Finperm n'} {b' : Finperm m'} (hab : a.IsCongr b)
     (hab' : a'.IsCongr b') : (a.hmul a').IsCongr (b.hmul b') :=
-  IsCongr.mul_mul (by grind) (by grind)
+  IsCongr.mul_mul (by simp [hab]) (by simp [hab'])
 
 grind_pattern IsCongr.hmul_hmul => a.hmul a', b.hmul b'
 
@@ -105,11 +138,9 @@ section MinPerm
 variable {n m : Nat} (a : Finperm n) (b : Finperm m)
 
 @[grind →] theorem IsCongr.minLen_eq (hab : a.IsCongr b) :
-    a.minLen = b.minLen := Nat.le_antisymm (by grind [isCongr_def]) (by grind [isCongr_def])
+    a.minLen = b.minLen := by rcases hab <;> grind
 
-@[simp] theorem isCongr_minPerm : a.IsCongr a.minPerm := by
-  simp only [isCongr_def, getElem_minPerm, implies_true, true_and]
-  exact ⟨a.getElem_eq_self_of_minLen_le, have := a.minLen_le; by omega⟩
+@[simp] theorem isCongr_minPerm : a.IsCongr a.minPerm := .inr ⟨a.minLen_le, a.minPerm_castGE⟩
 
 grind_pattern isCongr_minPerm => a.minPerm
 
@@ -119,6 +150,7 @@ grind_pattern minPerm_isCongr => a.minPerm
 
 @[simp] theorem isCongr_minPerm_left : a.minPerm.IsCongr b ↔ a.IsCongr b := by grind
 @[simp] theorem isCongr_minPerm_right : a.IsCongr b.minPerm ↔ a.IsCongr b := by grind
+
 theorem isCongr_minPerm_minPerm : a.minPerm.IsCongr b.minPerm ↔ a.IsCongr b := by simp
 
 theorem inv_minPerm_isCongr_inv : (a.minPerm)⁻¹.IsCongr a⁻¹ := (a.minPerm_isCongr).inv_inv
